Adapt nominal section to be more like dissertation

Tealeaves/Backends/Adapters/NominalToLN.v
@@ -1,10 +1,11 @@
 From Tealeaves Require Import
   Backends.LN
-  Backends.Nominal.Common
+  Backends.Nominal.Common.Hmap
+  Backends.Nominal.Common.Freshening
+  Backends.Nominal.Common.Binding
   Backends.Common.Names
   Backends.Nominal.FV
   Backends.Nominal.Alpha
-  Functors.Option
   LiftRel.TraversableFunctor
   Theory.DecoratedTraversableFunctorPoly
   CategoricalToKleisli.DecoratedFunctorPoly
@@ -72,8 +73,58 @@ Proof.
   reflexivity.
 Qed.
 
+(** ** Lemma About Mapdtp with Constant Applicatives *)
+(**********************************************************************)
+Section constant_applicatives.
 
+  Context
+    `{Categorical.DecoratedTraversableFunctorPoly.DecoratedTraversableFunctorPoly T}.
 
+  Context
+    {M} `{Monoid M}.
+
+  Import Categorical.TraversableFunctor2.
+  Import Adapters.PolyToMono.Categorical.TraversableFunctor.ToMono (dist2_natural_rw).
+  Import CategoricalToKleisli.DecoratedTraversableFunctorPoly.DerivedOperations.
+  Import CategoricalToKleisli.DecoratedTraversableFunctorPoly.DerivedInstances.
+
+  Lemma mapdtp_const1:
+    forall {A1 B1: Type} (A2 B2: Type) `(g: list B1 * B1 -> M) `(f: list B1 * A1 -> M),
+      mapdtp (G := const M) (B2 := False) (A2 := False) g f =
+        mapdtp (G := const M) (B2 := B2) (A2 := A2) g f.
+  Proof.
+    intros.
+    change_left
+      (map (F := const M)
+         (A := T False False)
+         (B := T B2 A2)
+         (map2 (F := T) (B1 := False) (A1 := False) (B2 := B2) (A2 := A2) exfalso exfalso)
+         ∘ mapdtp (T := T) (G := const M) g f).
+    unfold mapdtp.
+    unfold DerivedOperations.Mapdtp_Categorical.
+    reassociate <- on left.
+    reassociate <- on left.
+    unfold compose.
+    ext t.
+    rewrite <- dist2_natural_rw.
+    compose near (decp t).
+    rewrite fun2_map_map.
+    fequal.
+  Qed.
+
+  Lemma mapdtp_const_normalize:
+    forall {A1 B1: Type} (A2 B2: Type) `(g: list B1 * B1 -> M) `(f: list B1 * A1 -> M),
+      mapdtp (G := const M) (B2 := B2) (A2 := A2) g f =
+        mapdtp (G := const M) (B2 := False) (A2 := False) g f.
+  Proof.
+    intros.
+    symmetry.
+    apply mapdtp_const1.
+  Qed.
+
+End constant_applicatives.
+
+(*
 (** * Single-Argument DTM Instance *)
 (**********************************************************************)
 Section DTM.
@@ -120,280 +171,7 @@ Section DTM.
     Admitted.
 
 End DTM.
-
-(** * Histories and Contexts *)
-(********************************************************************)
-Section to_name_from_history.
-
-  (** ** <<to_name_from_history>> *)
-  (** Perform one local binder renaming on a locally nameless binder occurrence, given the history (the names assigned
-    to binders higher in the tree) and the initial avoid set.  *)
-  (********************************************************************)
-  Definition to_name_from_history
-    (top_avoid: list name)
-    (p: list name * unit): name :=
-    match p with
-    | (history, u) =>
-        fresh (top_avoid ++ history)
-    end.
-
-  (** *** Rewriting Principles for <<to_name_from_history>> *)
-  (********************************************************************)
-  Section to_name_from_history_rw.
-
-    Context (avoid: list name).
-
-    Lemma to_name_from_history_nil (u: unit):
-      to_name_from_history avoid (@nil atom, u) = fresh avoid.
-    Proof.
-      cbn -[fresh].
-      rewrite List.app_nil_r.
-      reflexivity.
-    Qed.
-
-    Lemma to_name_from_history_pair (history: list atom) (u: unit):
-      to_name_from_history avoid (history, u) = fresh (avoid ++ history).
-    Proof.
-      reflexivity.
-    Qed.
-
-    Lemma to_name_from_history_preincr (history: list atom):
-      to_name_from_history avoid ⦿ history =
-        to_name_from_history (avoid ++ history).
-    Proof.
-      ext [w l].
-      unfold preincr, incr, compose.
-      rewrite to_name_from_history_pair.
-      unfold to_name_from_history.
-      unfold_ops @Monoid_op_list.
-      rewrite <- List.app_assoc.
-      reflexivity.
-    Qed.
-
-  End to_name_from_history_rw.
-
-  (** *** Freshness for <<to_name_from_history>> *)
-  (********************************************************************)
-  Lemma to_name_from_history_fresh (avoid: list name): forall p,
-      ~ (to_name_from_history avoid p ∈ avoid).
-  Proof.
-    intros.
-    unfold to_name_from_history.
-    destruct p.
-    specialize (fresh_not_in (avoid ++ l)).
-    intros hyp contra.
-    apply hyp.
-    rewrite element_of_list_app.
-    now left.
-  Qed.
-
-  (** ** <<to_history_from_ctx>> *)
-  (** Given a locally nameless binding context (a list of unit values, representing its length-many binders in scope),
-    convert the context into same-length list of names assigned to each binder, given a top-level avoid set. *)
-  (********************************************************************)
-  Definition to_history_from_ctx (avoid: list name):
-    list unit -> list name :=
-    fold_with_history (to_name_from_history avoid).
-
-  Ltac fold_folds :=
-    repeat change (fold_with_history (to_name_from_history ?avoid)) with
-      (to_history_from_ctx avoid) in *.
-
-  (** *** Basic Properties of <<to_history_from_ctx>> *)
-  (********************************************************************)
-  Corollary length_to_history_from_ctx (avoid: list name) (l: list unit):
-    length (to_history_from_ctx avoid l) = length l.
-  Proof.
-    intros.
-    unfold to_history_from_ctx.
-    rewrite length_fold_with_history.
-    reflexivity.
-  Qed.
-
-  (** *** Rewriting Principles for <<to_history_from_ctx>> *)
-  (********************************************************************)
-  Section to_name_from_history_rw.
-
-    Context (avoid: list name).
-
-    Lemma to_history_from_ctx_nil:
-      to_history_from_ctx avoid nil = nil.
-    Proof.
-      reflexivity.
-    Qed.
-
-    Lemma to_history_from_ctx_cons (u: unit) (pre: list unit):
-      to_history_from_ctx avoid (u :: pre) =
-        fresh avoid :: to_history_from_ctx (avoid ++ [fresh avoid]) pre.
-    Proof.
-      unfold to_history_from_ctx.
-      rewrite fold_with_history_cons.
-      fequal.
-      - rewrite to_name_from_history_nil.
-        reflexivity.
-      - rewrite to_name_from_history_nil.
-        fequal.
-        ext [x y].
-        unfold preincr, incr, compose.
-        unfold_ops @Monoid_op_list.
-        unfold to_name_from_history.
-        rewrite List.app_assoc.
-        reflexivity.
-    Qed.
-
-    Lemma to_history_from_ctx_preincr
-      (history: list atom):
-      fold_with_history (to_name_from_history avoid ⦿ history) =
-        to_history_from_ctx (avoid ++ history).
-    Proof.
-      ext l.
-      generalize dependent avoid.
-      generalize dependent history.
-      induction l; intros.
-      - cbn.
-        reflexivity.
-      - rewrite fold_with_history_cons.
-        unfold to_history_from_ctx.
-        rewrite fold_with_history_cons.
-        fequal.
-        { unfold preincr, incr, compose.
-          change (history ● []) with (history ++ []).
-          rewrite List.app_nil_r.
-          cbn.
-          rewrite List.app_nil_r.
-          reflexivity.
-        }
-        { rewrite preincr_preincr.
-          rewrite IHl.
-          unfold to_history_from_ctx.
-          rewrite IHl.
-          change (?l1 ● ?l2) with (l1 ++ l2).
-          unfold to_history_from_ctx.
-          rewrite to_name_from_history_preincr.
-          rewrite List.app_assoc.
-          reflexivity.
-        }
-    Qed.
-
-  End to_name_from_history_rw.
-
-  (** *** Distributing <<to_history_from_ctx>> over a context *)
-  (********************************************************************)
-  (* Tailored for use when the list is a nominal binding context decomposition *)
-  Section to_history_from_ctx_decompose.
-
-    Context (avoid: list name) {l1 l2: list unit} {u: unit}.
-
-    Corollary to_history_from_ctx_decompose:
-      to_history_from_ctx avoid (l1 ++ [u] ++ l2) =
-        let init := to_history_from_ctx avoid l1 in
-        let mid := [to_name_from_history avoid (init , u)] in
-        let tail := to_history_from_ctx (avoid ++ init ++ mid) l2
-        in init ++ mid ++ tail.
-    Proof.
-      intros.
-      unfold to_name_from_history at 1.
-      unfold to_history_from_ctx.
-      rewrite fold_with_history_decompose.
-      rewrite to_history_from_ctx_preincr.
-      reflexivity.
-    Qed.
-
-  End to_history_from_ctx_decompose.
-
-  (** *** Freshness for <<to_history_from_ctx>> *)
-  (********************************************************************)
-  Lemma to_history_from_ctx_fresh (avoid: list name): forall (prefix: list unit),
-    forall (a: name),
-      a ∈ avoid ->
-      ~ a ∈ (to_history_from_ctx avoid prefix).
-  Proof.
-    introv Hin.
-    unfold to_name_from_history.
-    enough (cut: forall (x: atom), x ∈ to_history_from_ctx avoid prefix -> x <> a).
-    { intro contra.
-      specialize (cut a).
-      apply cut; auto.
-    }
-    apply fold_with_history_ind.
-    intros u h Hnotin.
-    specialize (to_name_from_history_fresh avoid (h, u)).
-    intro Hfresh.
-    intro contra.
-    subst. contradiction.
-  Qed.
-
-  (** ** <<to_name_from_ctx>> *)
-  (* give a name to a nameless binder in a context *)
-  (********************************************************************)
-  Definition to_name_from_ctx (avoid: list name):
-    list unit * unit -> name :=
-    run_using_prefix (to_name_from_history avoid).
-
-  (** *** Relation between <<to_history_from_ctx>> and <<to_name_from_ctx>> *)
-  (********************************************************************)
-  Lemma to_history_from_ctx_spec (avoid: list name):
-    to_history_from_ctx avoid =
-      mapdz (T := list) (to_name_from_ctx avoid).
-  Proof.
-    unfold to_name_from_ctx.
-    rewrite run_using_prefix_spec.
-    reflexivity.
-  Qed.
-
-  Lemma to_name_from_ctx_spec (avoid: list name) (ctx: list unit) (a: unit):
-    to_name_from_ctx avoid (ctx, a) =
-      to_name_from_history avoid (to_history_from_ctx avoid ctx, a).
-  Proof.
-    reflexivity.
-  Qed.
-
-  (** *** Rewriting rules for <<to_name_from_ctx>> *)
-  (********************************************************************)
-  Lemma to_name_from_ctx_rw_nil (avoid: list name): forall (u: unit),
-      to_name_from_ctx (avoid) (nil, u) =
-        fresh avoid.
-  Proof.
-    intros.
-    cbn.
-    rewrite List.app_nil_r.
-    reflexivity.
-  Qed.
-
-  Lemma to_name_from_ctx_rw_cons (avoid: list name): forall (u: unit) (rest: list unit) (u': unit),
-      to_name_from_ctx avoid (u :: rest, u') =
-        fresh (avoid ++ fresh avoid :: to_history_from_ctx (avoid ++ [fresh avoid]) rest).
-  Proof.
-    intros.
-    unfold to_name_from_ctx.
-    unfold run_using_prefix.
-    rewrite fold_with_history_cons.
-    unfold to_name_from_history at 1.
-    unfold to_name_from_history at 1.
-    rewrite List.app_nil_r.
-    rewrite to_history_from_ctx_preincr.
-    rewrite to_name_from_history_nil.
-    reflexivity.
-  Qed.
-
-  (** *** Freshness for <<to_name_from_ctx>> *)
-  (********************************************************************)
-  Lemma to_name_from_ctx_fresh (avoid: list name) (prefix: list unit) (u: unit):
-    ~ to_name_from_ctx avoid (prefix, u) ∈ avoid.
-  Proof.
-    intros.
-    unfold to_name_from_ctx.
-    intro contra.
-    unfold run_using_prefix in contra.
-    specialize (to_name_from_history_fresh avoid
-                  (fold_with_history (to_name_from_history avoid) prefix, u)).
-    intro Hyp.
-    apply Hyp.
-    assumption.
-  Qed.
-
-End to_name_from_history.
-
+*)
 
 (** * Converting a depth to (list unit) binding context *)
 (**********************************************************************)
@@ -402,6 +180,54 @@ Fixpoint length_to_list_unit (length: nat): list unit :=
   | 0 => nil
   | S n => tt :: length_to_list_unit n
   end.
+
+Lemma length_length_to_list_unit: forall n,
+    length (length_to_list_unit n) = n.
+Proof.
+  intros. induction n.
+  - reflexivity.
+  - cbn. fequal; auto.
+Qed.
+
+Lemma length_cons {A} {a:A} {l: list A}:
+  length (a :: l) = S (length l).
+Proof.
+  reflexivity.
+Qed.
+
+Lemma length_one {A} {a:A}:
+  length [a] = 1.
+Proof.
+  reflexivity.
+Qed.
+
+Lemma length_to_list_unit_plus {n m: nat}:
+  length_to_list_unit (n + m) =
+    length_to_list_unit n ++
+      length_to_list_unit m.
+Proof.
+  induction n.
+  - reflexivity.
+  - cbn. rewrite IHn.
+    reflexivity.
+Qed.
+
+Lemma length_to_list_unit_S (n: nat):
+  length_to_list_unit (S n) = tt :: length_to_list_unit n.
+Proof.
+  reflexivity.
+Qed.
+
+Lemma length_list_unit_iso (ctx: list unit):
+  ctx = length_to_list_unit (length ctx).
+Proof.
+  induction ctx.
+  - reflexivity.
+  - cbn. destruct a.
+    rewrite IHctx.
+    rewrite length_length_to_list_unit.
+    reflexivity.
+Qed.
 
 
 (** * Local Translations *)
@@ -471,57 +297,55 @@ Section with_DTM.
   Definition PANIC_INDEX_EXCEEDS_CONTEXT: nat := 1337.
 
   (* Give a DB index (Bd N), define its new name *)
-  Definition LN_BD_to_binder_name (avoid: list name) (ctx: list unit) (n: nat): atom :=
+  Definition bdToName (Γ: list name) (ctx: list unit) (n: nat): atom :=
     if Nat.ltb n (length ctx)
-    then to_name_from_ctx avoid (length_to_list_unit (length ctx - (n + 1)), tt)
+    then assignNames_loc Γ (length_to_list_unit (length ctx - (n + 1)), tt)
     else PANIC_INDEX_EXCEEDS_CONTEXT.
 
-  Lemma LN_BD_to_binder_name_fresh: forall avoid a ctx n,
+  Lemma bdToName_fresh: forall Γ a ctx n,
       length ctx > n ->
-      a ∈ avoid -> LN_BD_to_binder_name avoid ctx n <> a.
+      a ∈ Γ -> bdToName Γ ctx n <> a.
   Proof.
     introv Hlt Hin.
-    unfold LN_BD_to_binder_name.
+    unfold bdToName.
     apply PeanoNat.Nat.ltb_lt in Hlt.
     rewrite Hlt.
     intro contra.
     subst.
-    apply to_name_from_ctx_fresh in Hin.
+    apply assignNames_loc_fresh in Hin.
     assumption.
   Qed.
 
-  Definition ln_to_name (avoid: list name):
+  Definition lnToName (Γ: list name):
     list unit * LN -> name :=
     fun '(depth, v) =>
       match v with
       | Fr x => x
-      | Bd n => LN_BD_to_binder_name avoid depth n
+      | Bd n => bdToName Γ depth n
       end.
 
-  Definition term_ln_to_nominal (conflicts: list name):
+  Definition term_ln_to_nominal (Γ: list name):
     T unit LN -> T name name :=
-    mapdp (T := T)
-      (to_name_from_ctx conflicts)
-      (ln_to_name conflicts).
+    mapdp (T := T) (assignNames_loc Γ) (lnToName Γ).
 
-
-  (** ** Roundtrip Specifications *)
+  (** ** Roundtrip from Nominal *)
   (********************************************************************)
   (* The operation mapping a nominal term to a locally nameless term, then back again into a nominal term *)
-  Definition roundtrip_Nominal:
-    T name name -> T name name :=
-    fun t => let t_ln := term_nominal_to_ln t
-          in term_ln_to_nominal (LN.free t_ln) t_ln.
+  Definition rtFromNominal: T name name -> T name name :=
+    fun t =>
+      let t_ln := term_nominal_to_ln t
+      in term_ln_to_nominal (LN.free t_ln) t_ln.
 
-  Lemma roundtrip_Nominal_spec1:
+  Lemma rtFromNominal_spec:
     forall (t: T name name),
-      roundtrip_Nominal t =
-        mapdp
-          (kc_dz (to_name_from_ctx (free (term_nominal_to_ln t))) (const tt))
-          (kc_dfunp (ln_to_name (free (term_nominal_to_ln t))) (const tt) name_to_ln) t.
+      rtFromNominal t =
+        let Γ := free (term_nominal_to_ln t)
+        in mapdp
+             (kc_dz (assignNames_loc Γ) (const tt))
+             (kc_dfunp (lnToName Γ) (const tt) name_to_ln) t.
   Proof.
     intros.
-    unfold roundtrip_Nominal.
+    unfold rtFromNominal.
     compose near t on left.
     unfold term_nominal_to_ln at 2.
     unfold term_ln_to_nominal at 1.
@@ -529,80 +353,88 @@ Section with_DTM.
     reflexivity.
   Qed.
 
-  (** ** Decomposed into a Variable Op and Binder Op *)
+  (** ** Decomposed into a Variable Operation and Binder Operation *)
   (********************************************************************)
   (* Given a binding occurrence (pre, b) in a nominal term t,
      return the new name of b after a Nominal~>LN~>Nominal roundtrip *)
-  Section avoid.
+  Section roundtrip_decompose.
 
-    Context (avoid: list atom).
+    Context (Γ: list atom).
 
     Definition roundtrip_Binder_loc: Z atom -> atom :=
-      to_name_from_ctx avoid ∘ map (const tt).
+      assignNames_loc Γ ∘ map (const tt).
 
     (* Given a variable occurrence (pre, v) in a nominal term t,
      return the new name of v after a Nominal~>LN~>Nominal roundtrip *)
     Definition roundtrip_Var_loc: Z2 atom atom -> atom :=
-      kc_dfunp (ln_to_name avoid) (const tt) name_to_ln.
+      kc_dfunp (lnToName Γ) (const tt) name_to_ln.
 
     Lemma roundtrip_Binder_loc_spec:
       mapdz (T := list) roundtrip_Binder_loc =
-        to_history_from_ctx avoid ∘ map (const tt).
+        assignNames Γ ∘ map (const tt).
     Proof.
       intros.
       unfold roundtrip_Binder_loc.
-      rewrite to_history_from_ctx_spec.
+      rewrite assignNames_spec.
       Set Keyed Unification.
       rewrite (mapdz_map_list (A' := atom) (B := atom) (A := unit)).
       Unset Keyed Unification.
       reflexivity.
     Qed.
 
-  End avoid.
+  End roundtrip_decompose.
 
-  Lemma roundtrip_Nominal_spec_decomposed:
+  Lemma rtFromNominal_spec_decomposed:
     forall (t: T name name),
-      roundtrip_Nominal t =
-        let avoid := LN.free (term_nominal_to_ln t)
-        in rename_binders
-             (roundtrip_Binder_loc avoid)
-             (mapd (T := T name) (roundtrip_Var_loc avoid) t).
+      rtFromNominal t =
+        let Γ := LN.free (term_nominal_to_ln t)
+        in rename_binders (roundtrip_Binder_loc Γ)
+             (mapd (T := T name) (roundtrip_Var_loc Γ) t).
   Proof.
     intros.
-    rewrite roundtrip_Nominal_spec1.
+    rewrite rtFromNominal_spec.
     unfold kc_dz.
     rewrite cobind_Z_const.
     rewrite mapd_decompose.
     reflexivity.
   Qed.
 
-  (** *** Roundtrip effect on context occurrences *)
-  (* if (ctx, a) ∈d t, then (roundtrip_Occ (free t) (ctx, a)) ∈d roundtrip t *)
+  (** ** Roundtrip effect on context occurrences *)
+  (* if (ctx, a) ∈d t, then (rtFromNominal_occ (free t) (ctx, a)) ∈d roundtrip t *)
   (********************************************************************)
-  Definition roundtrip_Occ (avoid: list atom): list atom * atom -> list atom * atom :=
+  Definition rtFromNominal_occ (Γ: list atom):
+    list atom * atom -> list atom * atom :=
     fun '(ctx, a) =>
-      (mapdz (roundtrip_Binder_loc avoid) ctx, roundtrip_Var_loc avoid (ctx, a)).
+      (mapdz (roundtrip_Binder_loc Γ) ctx, roundtrip_Var_loc Γ (ctx, a)).
 
-  Lemma roundtrip_Occ_spec (avoid: list atom): forall ctx a,
-      roundtrip_Occ avoid (ctx, a) =
-        (map_fst (mapdz (T := list) (roundtrip_Binder_loc avoid))
-           (cobind (W := prod (list atom)) (roundtrip_Var_loc avoid) (ctx, a))).
+  Lemma rtFromNominal_occ_spec (Γ: list atom): forall ctx a,
+      rtFromNominal_occ Γ (ctx, a) =
+        (map_fst (mapdz (T := list) (roundtrip_Binder_loc Γ))
+           (cobind (W := prod (list atom)) (roundtrip_Var_loc Γ) (ctx, a))).
   Proof.
     intros.
-    unfold roundtrip_Occ.
+    unfold rtFromNominal_occ.
     unfold cobind.
     reflexivity.
   Qed.
 
-  Lemma roundtrip_Nominal_var_spec {avoid: list atom}:
+  Lemma rtFromNominal_occ_spec_pw: forall (Γ: list atom) (ctx: list atom) (a: atom),
+      rtFromNominal_occ Γ (ctx, a) =
+        (mapdz (roundtrip_Binder_loc Γ) ctx, roundtrip_Var_loc Γ (ctx, a)).
+  Proof.
+    unfold rtFromNominal_occ.
+    reflexivity.
+  Qed.
+
+  Lemma rtFromNominal_var_spec {Γ: list atom}:
     (kc_dfunp
-       (ln_to_name avoid)
+       (lnToName Γ)
        (const tt)
        name_to_ln) =
       fun '(ctx, nm) =>
         match binding_to_ln (get_binding ctx nm) with
         | Fr x => x
-        | Bd n => LN_BD_to_binder_name avoid (map (const tt) ctx) n
+        | Bd n => bdToName Γ (map (const tt) ctx) n
         end.
   Proof.
     ext [ctx nm].
@@ -619,7 +451,7 @@ Section with_DTM.
     reflexivity.
   Qed.
 
-  (** ** Deleting Binders *)
+  (** ** Specification for Decoration After Renaming Binders *)
   (********************************************************************)
   Lemma decorate_rename_binders {B1 B2 V}:
     forall (ρ: list B1 * B1 -> B2) (t: T B1 V),
@@ -628,6 +460,7 @@ Section with_DTM.
   Proof.
     intros.
     unfold delete_binders.
+    unfold bmap.
     unfold_ops @Map2_1.
     unfold_ops @Map2_2.
     unfold_ops @Decorate_PolyVar.
@@ -682,15 +515,20 @@ Section with_DTM.
     rewrite decorate_rename_binders.
     compose near (dec (T B1) t).
     unfold delete_binders.
+    unfold bmap.
     rewrite fun2_map22_map21_commute.
     reflexivity.
   Qed.
 
+
+  (** *** Occurence Relation After Deleting Binders *)
+  (********************************************************************)
   Lemma in_del_binders {B A}: forall (t: T B A) (a: A),
       element_of a (delete_binders t) = element_of a t.
   Proof.
     intros.
     unfold delete_binders.
+    unfold bmap.
     unfold element_of.
     rewrite tosubset_to_foldMap.
     rewrite tosubset_to_foldMap.
@@ -704,53 +542,6 @@ Section with_DTM.
     rewrite Dist2_1_natural2.
     reflexivity.
   Qed.
-
-
-  (** ** Lemma About Mapdtp with Constant Applicatives *)
-  (**********************************************************************)
-  Section constant_applicatives.
-
-    Context
-      {M} `{Monoid M}.
-
-    Import Categorical.TraversableFunctor2.
-
-    Lemma mapdtp_const1:
-      forall {A1 B1: Type} (A2 B2: Type) `(g: list B1 * B1 -> M) `(f: list B1 * A1 -> M),
-        mapdtp (G := const M) (B2 := False) (A2 := False) g f =
-          mapdtp (G := const M) (B2 := B2) (A2 := A2) g f.
-    Proof.
-      intros.
-      change_left
-        (map (F := const M)
-           (A := T False False)
-           (B := T B2 A2)
-           (map2 (F := T) (B1 := False) (A1 := False) (B2 := B2) (A2 := A2) exfalso exfalso)
-           ∘ mapdtp (T := T) (G := const M) g f).
-      unfold mapdtp.
-      unfold DerivedOperations.Mapdtp_Categorical.
-      reassociate <- on left.
-      reassociate <- on left.
-      unfold compose.
-      ext t.
-      rewrite <- dist2_natural_rw.
-      compose near (decp t).
-      rewrite fun2_map_map.
-      fequal.
-    Qed.
-
-
-    Lemma mapdtp_const_normalize:
-      forall {A1 B1: Type} (A2 B2: Type) `(g: list B1 * B1 -> M) `(f: list B1 * A1 -> M),
-        mapdtp (G := const M) (B2 := B2) (A2 := A2) g f =
-          mapdtp (G := const M) (B2 := False) (A2 := False) g f.
-    Proof.
-      intros.
-      symmetry.
-      apply mapdtp_const1.
-    Qed.
-
-  End constant_applicatives.
 
   (** ** Relating Free Variables During Translation *)
   (********************************************************************)
@@ -769,16 +560,12 @@ Section with_DTM.
     change (id ∘ ?f) with f.
     change (f ∘ ?id) with f.
     change_left ((mapdtp (B2 := atom) (A2 := False) (B1 := atom) (A1 := atom) (pure (F := const M)) f) t).
-    pose @mapdtp_const_normalize.
-    specialize (e M _ _ H3).
-    specialize (e atom atom False atom).
-    rewrite e.
-    clear e.
-    pose @mapdtp_const_normalize.
-    specialize (e M _ _ H3).
-    specialize (e atom atom False unit).
-    rewrite e.
-    clear e.
+    pose (cut := mapdtp_const_normalize False (A1 := atom) (B1 := atom) atom).
+    rewrite cut.
+    clear cut.
+    pose (cut := mapdtp_const_normalize False (A1 := atom) (B1 := atom) unit).
+    rewrite cut.
+    clear cut.
     reflexivity.
   Qed.
 
@@ -801,7 +588,7 @@ Section with_DTM.
     change (?x ∘ id) with x; change (id ∘ ?x) with x.
     unfold compose.
     compose near (decp t).
-    rewrite (fun2_map_map).
+    rewrite fun2_map_map.
     rewrite normalize_foldMap.
     unfold mapdtp.
     unfold DerivedOperations.Mapdtp_Categorical.
@@ -810,7 +597,7 @@ Section with_DTM.
     { ext [l v].
       unfold compose.
       unfold name_to_ln.
-      destruct (get_binding_spec l v) as [[Hbinding Hspec] | [pre [post [Hbinding [Hspec1 Hspec2]]]]].
+      destruct (get_binding_spec_proof l v) as [[Hbinding Hspec] | [pre [post [Hbinding [Hspec1 Hspec2]]]]].
       - cbn.
         rewrite Hbinding.
         reflexivity.
@@ -824,34 +611,24 @@ Section with_DTM.
 
   (** ** Alpha Equivalence Local Reasoning *)
   (********************************************************************)
-  Lemma to_name_from_ctx_preincr: forall avoid a,
-      to_name_from_ctx avoid ∘ cobind (W := Z) (const tt) ∘ incr [a] =
-        to_name_from_ctx (avoid ++ [fresh avoid]) ∘ cobind (const tt).
+  Lemma assignNames_loc_preincr: forall Γ a,
+      assignNames_loc Γ ∘ cobind (W := Z) (const tt) ∘ incr [a] =
+        assignNames_loc (Γ ++ [fresh Γ]) ∘ cobind (const tt).
   Proof.
     intros.
     ext [ctx x].
     unfold compose.
-    unfold to_name_from_ctx.
+    unfold assignNames_loc.
   Abort.
 
-  (** *** Specification of <<roundtrip_Occ>> *)
+  (** *** Specification of <<rtFromNominal_occ>> when a is unbound *)
   (********************************************************************)
-  Lemma roundtrip_Occ_spec_pw: forall (avoid: list atom) (ctx: list atom) (a: atom),
-      roundtrip_Occ avoid (ctx, a) =
-        (mapdz (roundtrip_Binder_loc avoid) ctx, roundtrip_Var_loc avoid (ctx, a)).
-  Proof.
-    unfold roundtrip_Occ.
-    reflexivity.
-  Qed.
-
-  (** *** Specification of <<roundtrip_Occ>> when a is unbound *)
-  (********************************************************************)
-  Lemma roundtrip_Occ_Unbound_spec: forall (avoid: list atom) (ctx: list atom) (a: atom),
+  Lemma rtFromNominal_occ_Unbound_spec: forall (Γ: list atom) (ctx: list atom) (a: atom),
       get_binding ctx a = Unbound ctx a ->
-      roundtrip_Occ avoid (ctx, a) = (mapdz (roundtrip_Binder_loc avoid) ctx, a).
+      rtFromNominal_occ Γ (ctx, a) = (mapdz (roundtrip_Binder_loc Γ) ctx, a).
   Proof.
     introv Hyp.
-    rewrite roundtrip_Occ_spec_pw.
+    rewrite rtFromNominal_occ_spec_pw.
     fequal.
     cbn.
     rewrite Hyp.
@@ -860,15 +637,15 @@ Section with_DTM.
 
   (** *** Specification of <<roundtrip_Var_loc>> when a is bound *)
   (********************************************************************)
-  Lemma roundtrip_Var_loc_Bound_spec: forall (avoid: list atom) (ctx: list atom) (a: atom) prefix a' postfix,
+  Lemma roundtrip_Var_loc_Bound_spec: forall (Γ: list atom) (ctx: list atom) (a: atom) prefix a' postfix,
       get_binding ctx a = Bound prefix a' postfix ->
       ctx = prefix ++ [a'] ++ postfix ->
       a = a' ->
-      roundtrip_Var_loc avoid (ctx, a) =
-        to_name_from_history avoid (to_history_from_ctx avoid (map (const tt) prefix), tt).
+      roundtrip_Var_loc Γ (ctx, a) =
+        historyToName Γ (assignNames Γ (map (const tt) prefix), tt).
   Proof.
     introv Hbinding Hctx Haeq.
-    unfold to_name_from_history.
+    unfold historyToName.
     unfold roundtrip_Var_loc.
     unfold kc_dfunp.
     rewrite cobind_Z2_const.
@@ -877,8 +654,8 @@ Section with_DTM.
     rewrite Haeq in *; clear Haeq.
     rewrite Hbinding.
     unfold binding_to_ln.
-    unfold ln_to_name.
-    unfold LN_BD_to_binder_name.
+    unfold lnToName.
+    unfold bdToName.
     rewrite map_preserve_length.
     assert (HsafeIx: length postfix < length ctx).
     { subst.
@@ -889,12 +666,12 @@ Section with_DTM.
     }
     rewrite <- PeanoNat.Nat.ltb_lt in HsafeIx.
     rewrite HsafeIx.
-    unfold to_name_from_ctx.
-    unfold run_using_prefix.
-    unfold to_name_from_history.
+    unfold assignNames_loc.
+    unfold hadapt.
+    unfold historyToName.
     fequal.
     fequal.
-    unfold to_history_from_ctx.
+    unfold assignNames.
     fequal.
     assert (Hineq: length ctx - (length postfix + 1) = length prefix).
     { subst.
@@ -909,27 +686,27 @@ Section with_DTM.
       - cbn. now rewrite IHprefix. }
   Qed.
 
-  (** *** Specification of <<get_binding ∘ roundtrip_Occ>> when a is unbound *)
+  (** *** Specification of <<get_binding ∘ rtFromNominal_occ>> when a is unbound *)
   (********************************************************************)
-  Lemma roundtrip_Occ_get_binding_Unbound_spec:
-    forall (avoid: list atom) (ctx: list atom) (a: atom),
-      a ∈ avoid ->
+  Lemma rtFromNominal_occ_get_binding_Unbound_spec:
+    forall (Γ: list atom) (ctx: list atom) (a: atom),
+      a ∈ Γ ->
       get_binding ctx a = Unbound ctx a ->
-      match roundtrip_Occ avoid (ctx, a) with
+      match rtFromNominal_occ Γ (ctx, a) with
       | (foo, x) =>
-          get_binding foo x = Unbound (mapdz (roundtrip_Binder_loc avoid) ctx) a
+          get_binding foo x = Unbound (mapdz (roundtrip_Binder_loc Γ) ctx) a
       end.
   Proof.
     introv Hnin Hyp.
-    rewrite roundtrip_Occ_Unbound_spec; auto.
-    destruct (get_binding_spec (mapdz (roundtrip_Binder_loc avoid) ctx) a)
+    rewrite rtFromNominal_occ_Unbound_spec; auto.
+    destruct (get_binding_spec_proof (mapdz (roundtrip_Binder_loc Γ) ctx) a)
       as [[Case1 rest] | [prefix [postfix [Case2 [ctxspec Hnin']]]]].
     { rewrite Case1.
       reflexivity. }
-    { assert (Hfresh: ~ a ∈ mapdz (roundtrip_Binder_loc avoid) ctx).
+    { assert (Hfresh: ~ a ∈ mapdz (roundtrip_Binder_loc Γ) ctx).
       { rewrite roundtrip_Binder_loc_spec.
         unfold compose at 1.
-        apply to_history_from_ctx_fresh.
+        apply assignNames_fresh.
         assumption.
       }
       apply get_binding1 in Hfresh.
@@ -937,33 +714,33 @@ Section with_DTM.
     }
   Qed.
 
-  (** *** Specification of <<get_binding ∘ roundtrip_Occ>> when a is bound *)
+  (** *** Specification of <<get_binding ∘ rtFromNominal_occ>> when a is bound *)
   (********************************************************************)
-  Lemma roundtrip_Occ_get_binding_Bound_spec:
-    forall (avoid: list atom) (ctx: list atom) (a: atom) prefix a' postfix,
+  Lemma rtFromNominal_occ_get_binding_Bound_spec:
+    forall (Γ: list atom) (ctx: list atom) (a: atom) prefix a' postfix,
       get_binding ctx a = Bound prefix a' postfix ->
       a = a' ->
       ctx = prefix ++ [a'] ++ postfix ->
       ~ a ∈ postfix ->
-      match roundtrip_Occ avoid (ctx, a) with
+      match rtFromNominal_occ Γ (ctx, a) with
       | (foo, x) =>
-          let NewPrefix := to_history_from_ctx avoid (map (const tt) prefix)
-          in let NewVar := to_name_from_history avoid (NewPrefix, tt)
-             in let NewPost := to_history_from_ctx (avoid ++ NewPrefix ++ [NewVar]) (map (const tt) postfix)
+          let NewPrefix := assignNames Γ (map (const tt) prefix)
+          in let NewVar := historyToName Γ (NewPrefix, tt)
+             in let NewPost := assignNames (Γ ++ NewPrefix ++ [NewVar]) (map (const tt) postfix)
                 in get_binding foo x = Bound NewPrefix NewVar NewPost /\ length NewPrefix = length prefix
       end.
   Proof.
     introv Hyp Haeq Hctxeq Hnin.
-    remember (roundtrip_Occ avoid (ctx, a)).
+    remember (rtFromNominal_occ Γ (ctx, a)).
     destruct p.
-    rewrite roundtrip_Occ_spec_pw in Heqp.
+    rewrite rtFromNominal_occ_spec_pw in Heqp.
     injection Heqp; introv Hctx' HVar'.
     clear Heqp.
     intros NewPrefix NewVar NewPost.
     split.
     { assert
         (HRoundtripMapsToNewVar:
-          roundtrip_Var_loc avoid (prefix ++ [a'] ++ postfix, a') = NewVar).
+          roundtrip_Var_loc Γ (prefix ++ [a'] ++ postfix, a') = NewVar).
       { subst.
         unfold NewVar.
         unfold NewPrefix.
@@ -979,13 +756,13 @@ Section with_DTM.
         rewrite map_list_app.
         rewrite map_list_one.
         change (const tt a') with tt.
-        rewrite to_history_from_ctx_decompose.
+        rewrite assignNames_decompose.
         fold NewPrefix.
         fold NewVar.
         fold NewPost.
         rewrite HRoundtripMapsToNewVar.
         reflexivity.
-      - apply to_history_from_ctx_fresh.
+      - apply assignNames_fresh.
         rewrite element_of_list_app.
         rewrite element_of_list_app.
         right; right.
@@ -994,37 +771,37 @@ Section with_DTM.
         assumption.
     }
     { unfold NewPrefix.
-      rewrite length_to_history_from_ctx.
+      rewrite length_assignNames.
       rewrite map_preserve_length.
       reflexivity.
     }
   Qed.
 
   Lemma rt_correct_local2:
-    forall (t: T name name) (avoid: list name)
-      (Havoidinit: forall (a: name), (a ∈ FV t -> a ∈ avoid)),
+    forall (t: T name name) (Γ: list name)
+      (HΓinit: forall (a: name), (a ∈ FV t -> a ∈ Γ)),
     forall (ctx: list name) (a: name),
       (ctx, a) ∈ (dec (T atom) t) ->
-      alpha_equiv_local (ctx, a) (roundtrip_Occ avoid (ctx, a)).
+      alpha_equiv_local (ctx, a) (rtFromNominal_occ Γ (ctx, a)).
   Proof.
     introv HFV.
     introv Hin.
     unfold alpha_equiv_local.
-    destruct (get_binding_spec ctx a) as [[Case1 Hanin] | [prefix [postfix [Case2 [ctxspec Hnin]]]]].
+    destruct (get_binding_spec_proof ctx a) as [[Case1 Hanin] | [prefix [postfix [Case2 [ctxspec Hnin]]]]].
     { rewrite Case1.
-      assert (Havoid: a ∈ avoid).
+      assert (HΓ: a ∈ Γ).
       { apply HFV.
         apply (FV_lift_local _ ctx); auto.
       }
-      specialize (roundtrip_Occ_get_binding_Unbound_spec avoid ctx a Havoid Case1).
+      specialize (rtFromNominal_occ_get_binding_Unbound_spec Γ ctx a HΓ Case1).
       intro X.
-      destruct (roundtrip_Occ avoid (ctx, a)).
+      destruct (rtFromNominal_occ Γ (ctx, a)).
       rewrite X. destruct_eq_args a a.
     }
     {
       rewrite Case2.
-      apply (roundtrip_Occ_get_binding_Bound_spec avoid) in Case2; auto.
-      destruct (roundtrip_Occ avoid (ctx, a)).
+      apply (rtFromNominal_occ_get_binding_Bound_spec Γ) in Case2; auto.
+      destruct (rtFromNominal_occ Γ (ctx, a)).
       destruct Case2 as [Case2RW Case2Len].
       rewrite Case2RW.
       rewrite Case2Len.
@@ -1044,7 +821,7 @@ Section with_DTM.
     intros [ctx a].
     rewrite in_del_binders.
     unfold compose, precompose.
-    rewrite <- roundtrip_Occ_spec.
+    rewrite <- rtFromNominal_occ_spec.
     apply rt_correct_local2.
     clear a.
     introv HinFV.
@@ -1052,48 +829,50 @@ Section with_DTM.
     assumption.
   Qed.
 
-  Theorem roundtrip_correct: forall (t: T name name),
-      polymorphic_alpha T t (roundtrip_Nominal t).
+  (** ** Correctness of <<rtFromNominal>> *)
+  (********************************************************************)
+  Theorem rtFromNominal_correct: forall (t: T name name),
+      polymorphic_alpha T t (rtFromNominal t).
   Proof.
     intros.
-    rewrite (roundtrip_Nominal_spec_decomposed).
+    rewrite (rtFromNominal_spec_decomposed).
     unfold polymorphic_alpha.
-    unfold lift_relation_ctx_poly.
+    unfold lift_relation_ctx2.
     rewrite (decorate_rename_binders2).
     rewrite TraversableFunctor.relation_natural2.
     rewrite (CategoricalToKleisli.DecoratedFunctor.dec_mapd2 (list atom) (F := T atom)).
-    rewrite delete_binders_map.
+    change (map (F := ?F) (A := ?A) (B := ?B)) with (vmap (B := atom) (V1 := A) (V2 := A)).
+    rewrite delete_binders_vmap.
+    unfold vmap.
     rewrite relation_natural2.
     apply relation_diagonal1.
     apply rt_correct_local1.
   Qed.
 
-
-  Theorem roundtrip_correct2: forall (t: T name name),
+  Theorem rtFromNominal_correct2: forall (t: T name name),
       polymorphic_alpha T t (term_ln_to_nominal (free (term_nominal_to_ln t)) (term_nominal_to_ln t)).
   Proof.
     intros.
-    unfold roundtrip_Nominal.
-    apply roundtrip_correct.
+    unfold rtFromNominal.
+    apply rtFromNominal_correct.
   Qed.
-
-  Print Assumptions roundtrip_correct.
 
   (** ** Roundtrip in the Other Direction *)
   (********************************************************************)
-  Definition roundtrip_LN:
+  Definition rtFromLN:
     T unit LN -> T unit LN :=
-    fun t => let t_nom := term_ln_to_nominal (LN.free t) t
-          in term_nominal_to_ln t_nom.
+    fun t =>
+      let t_nom := term_ln_to_nominal (LN.free t) t
+      in term_nominal_to_ln t_nom.
 
-  Lemma roundtrip_LN_spec1:
+  Lemma rtFromLN_spec1:
     forall (t: T unit LN),
-      roundtrip_LN t =
-        mapdp (kc_dz (const tt) (to_name_from_ctx (free t)))
-          (kc_dfunp name_to_ln (to_name_from_ctx (free t)) (ln_to_name (free t))) t.
+      rtFromLN t =
+        mapdp (kc_dz (const tt) (assignNames_loc (free t)))
+          (kc_dfunp name_to_ln (assignNames_loc (free t)) (lnToName (free t))) t.
   Proof.
     intros.
-    unfold roundtrip_LN.
+    unfold rtFromLN.
     compose near t on left.
     unfold term_nominal_to_ln at 1.
     unfold term_ln_to_nominal at 1.
@@ -1101,37 +880,37 @@ Section with_DTM.
     reflexivity.
   Qed.
 
-  Lemma roundtrip_LN_spec_decomposed:
+  Lemma rtFromLN_spec_decomposed:
     forall (t: T unit LN),
-      roundtrip_LN t =
-        let avoid := free t
+      rtFromLN t =
+        let Γ := free t
         in (rename_binders (const tt)
            (mapd (T := T unit) (kc_dfunp (T := T)
                                   name_to_ln
-                                  (to_name_from_ctx avoid)
-                                  (ln_to_name avoid)) t)).
+                                  (assignNames_loc Γ)
+                                  (lnToName Γ)) t)).
   Proof.
     intros.
-    rewrite roundtrip_LN_spec1.
+    rewrite rtFromLN_spec1.
     unfold kc_dz.
-    change (const tt ∘ cobind (to_name_from_ctx (free t)))
+    change (const tt ∘ cobind (assignNames_loc (free t)))
       with (const (A := list unit * unit) tt).
     rewrite mapd_decompose.
     reflexivity.
   Qed.
 
-  Lemma roundtrip_LN_spec_decomposed2:
+  Lemma rtFromLN_spec_decomposed2:
     forall (t: T unit LN),
-      roundtrip_LN t =
-        let avoid := free t
+      rtFromLN t =
+        let Γ := free t
         in (mapd (T := T unit)
               (kc_dfunp (T := T)
                  name_to_ln
-                 (to_name_from_ctx avoid)
-                 (ln_to_name avoid)) t).
+                 (assignNames_loc Γ)
+                 (lnToName Γ)) t).
   Proof.
     intros.
-    rewrite roundtrip_LN_spec_decomposed.
+    rewrite rtFromLN_spec_decomposed.
     assert (Hren: rename_binders (V1 := LN) (T := T) (const tt (A := list unit * unit)) = id).
     { unfold rename_binders.
       assert (Hconst: const tt (A := list unit * unit) = extract).
@@ -1151,141 +930,241 @@ Section with_DTM.
 
   Import CategoricalToKleisli.DecoratedTraversableFunctor.DerivedOperations.
 
-  Lemma length_length_to_list_unit: forall n,
-      length (length_to_list_unit n) = n.
-  Proof.
-    intros. induction n.
-    - reflexivity.
-    - cbn. fequal; auto.
-  Qed.
 
-  Lemma get_binding_LN_rt2: forall (l: list atom) (ctx: list unit) (n: nat),
-      n < length ctx ->
-      (get_binding (to_history_from_ctx l ctx)
-         (to_name_from_ctx l (length_to_list_unit (length ctx - (n + 1)), tt))) =
-        Bound
-          (to_history_from_ctx l (length_to_list_unit (length ctx - (n + 1))))
-          (to_name_from_ctx l (length_to_list_unit (length ctx - (n + 1)), tt))
-          (to_history_from_ctx l (length_to_list_unit n)).
-  Proof.
-    introv Hlt.
-    induction ctx.
-    - false.
-      inversion Hlt.
-    - cbn in Hlt.
-      change (length (?x :: ?xs)) with (S (length xs)).
+  Section support.
+    Context (Γ: list atom).
 
-      admit.
-  Admitted.
+    Lemma get_binding_LN_rt2_lemma1: forall (ctx: list unit) (n: nat),
+        n < length ctx ->
+        ctx = (length_to_list_unit (length ctx - (n + 1)) ++ [ tt ]  ++ length_to_list_unit n).
+    Proof.
+      introv Hlt. induction ctx.
+      - false. cbn in Hlt. lia.
+      - compare naturals n and (length ctx).
+        + specialize (IHctx ineqp).
+          rewrite IHctx.
+          rewrite length_cons.
+          rewrite List.app_length.
+          rewrite length_length_to_list_unit.
+          rewrite List.app_length.
+          rewrite length_length_to_list_unit.
+          rewrite (length_one (a := tt)).
+          assert (HlenEq: (S (length ctx - (n + 1) + (1 + n)) - (n + 1)) = S (length ctx - (n + 1))).
+          { lia. }
+          rewrite HlenEq.
+          rewrite length_to_list_unit_S.
+          destruct a.
+          reflexivity.
+        + clear IHctx.
+          assert (HlenEq: (length (a :: ctx) - (length ctx + 1)) = 0).
+          { rewrite length_cons.
+            lia.
+          }
+          rewrite HlenEq.
+          destruct a.
+          rewrite <- length_list_unit_iso.
+          reflexivity.
+        + false. cbn in Hlt.
+          lia.
+    Qed.
 
-  Lemma get_binding_LN_rt1: forall (l: list atom) (ctx: list unit) (n: nat),
-      n < length ctx ->
-      binding_to_ln
-      (get_binding (to_history_from_ctx l ctx)
-         (to_name_from_ctx l (length_to_list_unit (length ctx - (n + 1)), tt))) =
-        Bd n.
-  Proof.
-    intros.
-    rewrite get_binding_LN_rt2; auto.
-    unfold binding_to_ln.
-    rewrite length_to_history_from_ctx.
-    rewrite length_length_to_list_unit.
-    reflexivity.
-  Qed.
+    #[local] Open Scope nat_scope.
 
-  Lemma decompose_list_by_ix: forall (A: Type) (l: list A) (n: nat),
-      n < length l ->
-      exists pre a post, l = pre ++ [a] ++ post /\
-                      length post = n.
-  Proof.
-    introv Hlt.
-    induction l.
-    - false.
-      inversion Hlt.
-    - cbn in Hlt.
-      compare naturals n and (length l).
-      { apply IHl in ineqp.
-        destruct ineqp as [pre [a' [post [Heq Hrest]]]].
-        exists (a :: pre) a' post; split; auto.
-        rewrite Heq.
-        rewrite List.app_comm_cons.
-        reflexivity.
-      }
-      { exists (@nil A)  a l.
-        rewrite List.app_nil_l.
-        auto.
-      }
-  Qed.
-
-  Lemma get_binding_LN_new2: forall (l: list atom) (pre: list unit) (post: list unit),
-      (get_binding
-         (to_history_from_ctx l pre ++
-            [to_name_from_history l (to_history_from_ctx l pre, tt)] ++
-            to_history_from_ctx
-            (l ++ to_history_from_ctx l pre ++ [to_name_from_history l (to_history_from_ctx l pre, tt)]) post)
-         (to_name_from_history l (to_history_from_ctx l pre, tt)))
-      =  Bound
-           (to_history_from_ctx l pre)
-           (to_name_from_history l (to_history_from_ctx l pre, tt))
-           (to_history_from_ctx
-              (l ++ to_history_from_ctx l pre ++ [to_name_from_history l (to_history_from_ctx l pre, tt)]) post).
-  Proof.
-    intros.
-    apply get_binding2.
-    - reflexivity.
-    - reflexivity.
-    - apply  to_history_from_ctx_fresh.
-      rewrite element_of_list_app.
-      rewrite element_of_list_app.
-      rewrite element_of_list_one.
-      right. right. reflexivity.
-  Qed.
-
-  Lemma get_binding_LN_new: forall (l: list atom) (ctx: list unit) (n: nat),
-      n < length ctx ->
-      binding_to_ln
-      (get_binding (to_history_from_ctx l ctx)
-         (to_name_from_ctx l (length_to_list_unit (length ctx - (n + 1)), tt))) =
-        Bd n.
-  Proof.
-    introv Hin.
-    apply decompose_list_by_ix in Hin.
-    destruct Hin as [pre [a [post [Heq Hlen]]]].
-    (*
-    intro cut.
-    rewrite Heq.
-    rewrite cut.
-    assert (Hlen_spec: length (pre ++ [a] ++ post) - (n + 1) = length pre).
-    { subst.
-      rewrite List.app_length.
-      rewrite List.app_length.
-      cbn.
+    Lemma nat_decompose: forall (ctx: nat) (part: nat),
+        part < ctx ->
+        ctx = part + 1 + (ctx - part - 1).
+    Proof.
+      introv Hlen.
       lia.
-    }
-    rewrite Hlen_spec.
-    rewrite to_name_from_ctx_spec.
+    Qed.
 
-    assert (Hpre: length_to_list_unit (length pre) = pre).
-    { admit. }
-    rewrite Hpre.
-    assert (Ha: a = tt).
-    { now destruct a. }
-    rewrite Ha.
-    rewrite get_binding_LN_new2.
-    unfold binding_to_ln.
-    rewrite length_to_history_from_ctx.
-    auto.
-   *)
+    Lemma list_unit_decompose: forall (ctx: list unit) (part: list unit),
+        length part < length ctx ->
+        ctx = part ++ [tt] ++ (length_to_list_unit (length ctx - length part - 1)).
+    Proof.
+      introv Hlen.
+      pose (Helper:= nat_decompose (length ctx) (length part) Hlen).
+      rewrite (length_list_unit_iso ctx) at 1.
+      rewrite (length_list_unit_iso part) at 1.
+      rewrite Helper.
+      clear Helper.
+      rewrite length_to_list_unit_plus.
+      rewrite List.app_assoc.
+      rewrite length_to_list_unit_plus.
+      fequal.
+      fequal. lia.
+    Qed.
+
+    Lemma get_binding_LN_rt2_generalized: forall (ctx: list unit) (part: list unit),
+        length part < length ctx ->
+        (get_binding (assignNames Γ ctx) (assignNames_loc Γ (part, tt))) =
+          Bound
+            (assignNames Γ part)
+            (assignNames_loc Γ (part, tt))
+            (assignNames (Γ ++ assignNames Γ part ++ [assignNames_loc Γ (part, tt)])
+               (length_to_list_unit (length ctx - length part - 1))).
+    Proof.
+      introv Hlt.
+      apply get_binding2.
+      - reflexivity.
+      - rewrite (list_unit_decompose ctx part); [| assumption].
+        rewrite assignNames_decompose.
+        cbn zeta.
+        rewrite assignNames_loc_spec.
+        fequal.
+        fequal.
+        fequal.
+        fequal.
+        do 2 rewrite List.app_length.
+        rewrite (length_one (a := tt)).
+        rewrite length_length_to_list_unit.
+        lia.
+      - apply assignNames_fresh.
+        simpl_list.
+        tauto.
+    Qed.
+
+    Lemma get_binding_LN_rt2: forall (ctx: list unit) (n: nat),
+        n < length ctx ->
+        (get_binding (assignNames Γ ctx)
+           (assignNames_loc Γ (length_to_list_unit (length ctx - (n + 1)), tt))) =
+          Bound
+            (assignNames Γ (length_to_list_unit (length ctx - (n + 1))))
+            (assignNames_loc Γ (length_to_list_unit (length ctx - (n + 1)), tt))
+            (assignNames (Γ ++ assignNames Γ (length_to_list_unit (length ctx - (n + 1))) ++
+                            [assignNames_loc Γ ((length_to_list_unit (length ctx - (n + 1))), tt)])
+               (length_to_list_unit n)).
+    Proof.
+      introv Hlt.
+      rewrite get_binding_LN_rt2_generalized.
+      - fequal.
+        fequal.
+        fequal.
+        rewrite length_length_to_list_unit.
+        lia.
+      - rewrite length_length_to_list_unit.
+        lia.
+    Qed.
+
+    Lemma get_binding_LN_rt1: forall (ctx: list unit) (n: nat),
+        n < length ctx ->
+        binding_to_ln
+          (get_binding (assignNames Γ ctx)
+             (assignNames_loc Γ (length_to_list_unit (length ctx - (n + 1)), tt))) =
+          Bd n.
+    Proof.
+      intros.
+      rewrite get_binding_LN_rt2; auto.
+      unfold binding_to_ln.
+      rewrite length_assignNames.
+      rewrite length_length_to_list_unit.
+      reflexivity.
+    Qed.
+
+    Lemma decompose_list_by_ix: forall (A: Type) (l: list A) (n: nat),
+        n < length l ->
+        exists pre a post, l = pre ++ [a] ++ post /\
+                        length post = n.
+    Proof.
+      introv Hlt.
+      induction l.
+      - false.
+        inversion Hlt.
+      - cbn in Hlt.
+        compare naturals n and (length l).
+        { apply IHl in ineqp.
+          destruct ineqp as [pre [a' [post [Heq Hrest]]]].
+          exists (a :: pre) a' post; split; auto.
+          rewrite Heq.
+          rewrite List.app_comm_cons.
+          reflexivity.
+        }
+        { exists (@nil A)  a l.
+          rewrite List.app_nil_l.
+          auto.
+        }
+    Qed.
+
+    Lemma get_binding_LN_new2: forall (l: list atom) (pre: list unit) (post: list unit),
+        (get_binding
+           (assignNames l pre ++
+              [historyToName l (assignNames l pre, tt)] ++
+              assignNames
+              (l ++ assignNames l pre ++ [historyToName l (assignNames l pre, tt)]) post)
+           (historyToName l (assignNames l pre, tt)))
+        =  Bound
+             (assignNames l pre)
+             (historyToName l (assignNames l pre, tt))
+             (assignNames
+                (l ++ assignNames l pre ++ [historyToName l (assignNames l pre, tt)]) post).
+    Proof.
+      intros.
+      apply get_binding2.
+      - reflexivity.
+      - reflexivity.
+      - apply  assignNames_fresh.
+        rewrite element_of_list_app.
+        rewrite element_of_list_app.
+        rewrite element_of_list_one.
+        right. right. reflexivity.
+    Qed.
+
+  End support.
+
+  Lemma rtFromLN_id_local:
+    forall (t : T unit LN) (HLC: LC t)
+      (FVt: list atom) (HeqFVt: FVt = free t)
+      (ctx: list unit) (v: LN) (Hin: (ctx, v) ∈d t),
+      binding_to_ln (get_binding (assignNames FVt ctx) (lnToName FVt (ctx, v))) = v.
+  Proof.
+    intros.
+    destruct v as [a | n].
+    - unfold lnToName.
+      assert (H_a_not_assigned: ~ a ∈ assignNames FVt ctx).
+      { apply assignNames_fresh.
+        subst.
+        admit. }
+      assert (H_get_binding_Unbound:
+               get_binding (assignNames FVt ctx) a = Unbound (assignNames FVt ctx) a).
+      { destruct (get_binding_spec_proof (assignNames FVt ctx) a)
+          as [[Case1 rest] | [prefix [postfix [Case2 [ctxspec Hnin']]]]].
+        - assumption.
+        - false. apply H_a_not_assigned.
+          subst. rewrite ctxspec.
+          simpl_list. tauto. }
+      rewrite H_get_binding_Unbound.
+      reflexivity.
+    - unfold lnToName.
+      unfold bdToName.
+      assert (H_n_lt: Nat.ltb n (length ctx) = true).
+      { rewrite OrdersEx.Nat_as_OT.ltb_lt.
+        unfold LC in HLC.
+        unfold LCn in HLC.
+        specialize (HLC (length ctx)).
+        specialize (HLC (Bd n)).
+        assert (cut: (length ctx, Bd n) ∈d t).
+        Unset Printing Notations.
+        Set Printing Implicit.
+        { admit. }
+        apply HLC in cut.
+        unfold lc_loc in cut.
+        lia.
+      }
+      rewrite H_n_lt.
+      rewrite get_binding_LN_rt1.
+      + reflexivity.
+      + rewrite <- OrdersEx.Nat_as_OT.ltb_lt.
+        assumption.
   Admitted.
 
-  Lemma roundtrip_LN_id: forall (t: T unit LN),
+  Lemma rtFromLN_id: forall (t: T unit LN),
       LC t ->
-      roundtrip_LN t = t.
+      rtFromLN t = t.
   Proof.
     introv HLC.
-    rewrite roundtrip_LN_spec_decomposed2.
-    remember (free t).
-    cbn zeta.
+    rewrite rtFromLN_spec_decomposed2.
+    remember (free t) as FVt.
+    cbn.
     apply mapd_respectful_id.
     intros ctx v Hin.
     unfold kc_dfunp.
@@ -1295,92 +1174,21 @@ Section with_DTM.
     compose near ctx on left.
     unfold_Z.
     rewrite <- mapd_list_prefix_spec.
-    change (mapd_list_prefix (to_name_from_ctx l) ctx)
-      with (mapdz (to_name_from_ctx l) ctx).
-    rewrite <- to_history_from_ctx_spec.
+    change (mapd_list_prefix (assignNames_loc FVt) ctx)
+      with (mapdz (assignNames_loc FVt) ctx).
+    rewrite <- assignNames_spec.
     unfold name_to_ln.
-    destruct v as [a | n].
-   - unfold ln_to_name.
-      destruct (get_binding_spec (to_history_from_ctx l ctx) a)
-        as [[Case1 rest] | [prefix [postfix [Case2 [ctxspec Hnin']]]]].
-      + rewrite Case1.
-        cbn.
-        reflexivity.
-      + specialize (to_history_from_ctx_fresh l) as lemma.
-        false.
-        assert (a_in_list: a ∈ l).
-        { subst.
-          admit.
-        }
-        specialize (lemma ctx a a_in_list).
-        subst.
-        rewrite ctxspec in lemma.
-        apply lemma.
-        rewrite element_of_list_app.
-        rewrite element_of_list_app.
-        right.
-        left.
-        rewrite element_of_list_one.
-        reflexivity.
-    - unfold ln_to_name.
-      unfold LN_BD_to_binder_name.
-      assert (H_n_lt: Nat.ltb n (length ctx) = true).
-      { rewrite OrdersEx.Nat_as_OT.ltb_lt.
-        unfold LC in HLC.
-        unfold LCn in HLC.
-        specialize (HLC (length ctx)).
-        specialize (HLC (Bd n)).
-        assert (cut: (length ctx, Bd n) ∈d t).
-        { admit. }
-        apply HLC in cut.
-        unfold lc_loc in cut.
-        lia.
-      }
-      rewrite H_n_lt.
-      rewrite get_binding_LN_rt1; auto.
-      rewrite <- OrdersEx.Nat_as_OT.ltb_lt.
-      assumption.
-  Admitted.
+    eapply rtFromLN_id_local; eauto.
+  Qed.
 
-
-  Lemma roundtrip_LN_correct: forall (t: T unit LN),
+  Lemma rtFromLN_correct: forall (t: T unit LN),
       LC t ->
       term_nominal_to_ln (term_ln_to_nominal (free t) t) = t.
   Proof.
     introv HLC.
-    unfold roundtrip_LN.
-    apply roundtrip_LN_id.
+    unfold rtFromLN.
+    apply rtFromLN_id.
     assumption.
   Qed.
-
-  Theorem correctness1: forall (t u: T name name),
-      term_nominal_to_ln t = term_nominal_to_ln u -> polymorphic_alpha T t u.
-  Proof.
-    introv Heq.
-    assert (cut1: polymorphic_alpha T t (term_ln_to_nominal (FV t) (term_nominal_to_ln t))).
-    { pose roundtrip_correct2.
-      rewrite FV_preserved.
-      admit.
-    }
-    assert (cut2: polymorphic_alpha T u (term_ln_to_nominal (FV u) (term_nominal_to_ln u))).
-    { pose roundtrip_correct2.
-      rewrite FV_preserved.
-      admit.
-    }
-    rewrite Heq in *.
-    assert (HFV: FV t = FV u).
-    { rewrite  FV_preserved.
-      rewrite  FV_preserved.
-      rewrite Heq.
-      reflexivity.
-    }
-    rewrite HFV in cut1.
-  Admitted.
-
-  Theorem correctness2: forall (t u: T name name),
-      polymorphic_alpha T t u -> term_nominal_to_ln t = term_nominal_to_ln u.
-  Proof.
-    introv Halpha.
-  Abort.
 
 End with_DTM.
