Tealeaves/Backends/Nominal/Barendregt.v
@@ -1,44 +1,8 @@
 From Tealeaves Require Import
-  Classes.EqDec_eq
-  Classes.Kleisli.DecoratedTraversableMonadPoly
-  Functors.List_Telescoping_General
-  Backends.Common.Names
-  Backends.Nominal.Common
+  Backends.Nominal.Common.Freshening
+  Backends.Nominal.Common.Binding
   Backends.Nominal.FV
-  Functors.Constant
-  Functors.Subset.
-
-Export Backends.Common.Names.
-Export Backends.Nominal.Common.
-
-Import Subset.Notations.
-Import Monoid.Notations.
-Import Applicative.Notations.
-Import List.ListNotations.
-Import Product.Notations.
-Import ContainerFunctor.Notations.
-
-Lemma destruct_in: forall (a: name) (l: list name),
-    a ∈ l \/ ~ (a ∈ l).
-Proof.
-  intros.
-  rewrite <- Name.name_inb_iff.
-  destruct (Name.name_inb a l); auto.
-Qed.
-
-Ltac step_set_test :=
-  match goal with
-  | H: ~ ?x ∈ ?t |- _ =>
-      let Hf := fresh "H" in
-      pose H as Hf;
-      rewrite <- Name.name_inb_iff_false in Hf;
-      progress (repeat rewrite Hf)
-  | H: ?x ∈ ?t |- _ =>
-      let Hf := fresh "H" in
-      pose H as Hf;
-      rewrite <- Name.name_inb_iff in Hf;
-      progress (repeat rewrite Hf)
-  end.
+  Kleisli.DecoratedTraversableMonadPoly.
 
 Section ops.
 
@@ -51,49 +15,35 @@ Section ops.
   Section rename_local.
 
     Context
+      (Γ: list name)
       (x: name)
       (u: T name name).
 
-    Context
-      (conflicts: list name)  (* Top level conflicts, intuitively {{x}} \cup FV t \cup FV u *).
-
-    Definition rename_binder_from_history {A}: list name * A -> name :=
-      fun '(history, _) => fresh (conflicts ++ history).
-
-    Definition context_to_history {A} (ctx : list A): list name :=
-      fold_with_history rename_binder_from_history ctx.
-
-    Definition rename_binder_from_context {B C}: list B * C -> name :=
-      fun '(ctx, v) => rename_binder_from_history (context_to_history ctx, v).
-
-    Definition subst_from_ctx:
+    Definition subst_loc:
       list name * name -> T name name :=
       fun '(ctx, v) =>
         match get_binding ctx v with
         | Unbound _ _ =>
-            (* v is a free variable *)
             if v == x
             then u
             else ret v
         | Bound prefix _ post =>
-            (* v is a bound variable, give it the name of whatever it was bound to *)
-            ret (rename_binder_from_context (prefix, v))
+            ret (renb_ctx Γ (prefix, v))
         end.
 
   End rename_local.
 
   Definition subst_top
+    (Γ: list name)
     (x: name) (u: T name name)
-    (conflicts: list name)
     (t: T name name): T name name :=
    substitute (G := fun A => A) (U := T)
-     (rename_binder_from_context conflicts)
-     (subst_from_ctx x u conflicts) t.
+     (renb_ctx Γ)
+     (subst_loc Γ x u) t.
 
   Definition subst
     (x: name) (u: T name name)
     (t: T name name): T name name :=
-
-    subst_top x u ([x] ++ FV t ++ FV u) t.
+    subst_top (FV t ++ FV u) x u t.
 
 End ops.
