Tealeaves/Backends/Nominal/Common/Hmap.v
@@ -1,0 +1,362 @@
+From Tealeaves Require Export
+  Functors.List_Telescoping_General
+  Functors.List.
+
+#[local] Open Scope list_scope.
+
+Import List.ListNotations.
+Import Monoid.Notations.
+Import ContainerFunctor.Notations.
+
+(** * The <<hmap>> Operation *)
+(**********************************************************************)
+(* Fold over a list of A's where each A has the prefix of the list so far *)
+Fixpoint hmap {A B: Type}
+  (f: list B * A -> B)
+  (l: list A): list B :=
+  match l with
+  | nil => nil
+  | cons a rest =>
+      f ([], a) :: hmap (f ⦿ [f ([], a)]) rest
+  end.
+
+(** ** Rewriting Rules for <<hmap>> *)
+(**********************************************************************)
+Section rw.
+
+  Context {A B: Type}.
+
+  Section basic.
+
+    Context (f: list B * A -> B).
+
+    Lemma hmap_nil:
+      hmap f nil = nil.
+    Proof.
+      reflexivity.
+    Qed.
+
+    Lemma hmap_cons {a l}:
+      hmap f (a :: l) =
+        f ([], a) :: hmap (f ⦿ [f ([], a)]) l.
+    Proof.
+      cbn.
+      reflexivity.
+    Qed.
+
+    Lemma hmap_one {a}:
+      hmap f ([a]) =
+        [f ([], a)].
+    Proof.
+      cbn.
+      reflexivity.
+    Qed.
+
+  End basic.
+
+  Lemma hmap_app {l1 l2: list A}:
+    forall (f: list B * A -> B),
+      hmap f (l1 ++ l2) =
+        hmap f l1 ++
+          hmap (f ⦿ hmap f l1) l2.
+  Proof.
+    induction l1 as [|a l1 IHl1]; intros.
+    - cbn. change (f ⦿ []) with (f ⦿ Ƶ).
+      now rewrite preincr_zero.
+    - rewrite <- List.app_comm_cons.
+      rewrite hmap_cons.
+      rewrite hmap_cons.
+      rewrite IHl1.
+      rewrite <- List.app_comm_cons.
+      rewrite preincr_preincr.
+      reflexivity.
+  Qed.
+
+  (* Tailored for use when the list is a nominal binding context decomposition *)
+  Lemma hmap_decompose {l1 l2: list A} {a: A}:
+    forall (f: list B * A -> B),
+      hmap f (l1 ++ [a] ++ l2) =
+        hmap f l1 ++
+          [f (hmap f l1, a)] ++
+          hmap (f ⦿ (hmap f l1 ++ [f (hmap f l1, a)])) l2.
+  Proof.
+    intros.
+    rewrite hmap_app.
+    rewrite hmap_app.
+    rewrite hmap_one.
+    rewrite preincr_preincr.
+    unfold preincr, incr, compose.
+    unfold_ops @Monoid_op_list.
+    rewrite List.app_nil_r.
+    reflexivity.
+  Qed.
+
+End rw.
+
+(** ** Preservation of <<length>> *)
+(**********************************************************************)
+Lemma length_hmap {A B}: forall (l: list A) (f: list B * A -> B),
+    length (hmap f l) = length l.
+Proof.
+  intros.
+  generalize dependent f.
+  induction l; intros.
+  - reflexivity.
+  - cbn. fequal.
+    apply IHl.
+Qed.
+
+(** ** An Induction Rule for <<hmap>> *)
+(**********************************************************************)
+Section induction.
+
+  Import Theory.TraversableFunctor.
+
+  Context
+    {A B: Type}
+    {f: list B * A -> B}
+    (P: B -> Prop).
+
+  Section Forall.
+
+    Context
+      (Hbase: forall (a: A), P (f (nil, a)))
+      (Hstep: forall (a: A) (h: list B),
+      Forall P h -> P (f (h, a))).
+
+    Lemma hmap_ind_Forall: forall (l: list A),
+        Forall P (hmap f l).
+    Proof.
+      intro l.
+      induction l as [| a rest IHrest] using List.rev_ind.
+      - reflexivity.
+      - rewrite hmap_app.
+        rewrite TraversableFunctor.forall_iff.
+        rewrite TraversableFunctor.forall_iff in IHrest.
+        intro b.
+        rewrite element_of_list_app.
+        intros [Case1| Case2].
+        + auto.
+        + rewrite hmap_one in Case2.
+          rewrite element_of_list_one in Case2.
+          subst.
+          apply Hstep.
+          change (@nil B) with (Ƶ: list B).
+          rewrite monoid_id_l.
+          rewrite TraversableFunctor.forall_iff.
+          assumption.
+    Qed.
+
+  End Forall.
+
+  Section elementwise.
+
+    Context
+      (Hbase: forall (a: A), P (f (nil, a)))
+      (Hstep: forall (a: A) (h: list B),
+      (forall (b: B), b ∈ h -> P b) -> P (f (h, a))).
+
+    Lemma hmap_ind: forall (l: list A),
+      forall (b: B), b ∈ hmap f l -> P b.
+    Proof.
+      intro l.
+      rewrite <- TraversableFunctor.forall_iff.
+      apply hmap_ind_Forall.
+      intros; apply Hstep.
+      rewrite TraversableFunctor.forall_iff in H.
+      assumption.
+    Qed.
+
+  End elementwise.
+
+End induction.
+
+(** * Relating History to the Prefix: <<hadapt>> *)
+(**********************************************************************)
+Definition hadapt {A B: Type} (f: list B * A -> B): list A * A -> B :=
+  fun '(prefix, a) => f (hmap f prefix, a).
+
+(** ** Rewriting Rules *)
+(**********************************************************************)
+Section relate_history_prefix.
+
+  Context {A B: Type} (f: list B * A -> B).
+
+  (** *** Spec for <<scons>> *)
+  (**********************************************************************)
+  Lemma hadapt_app_one_spec: forall (l: list A) (a: A),
+      hmap f (l ++ [a]) =
+        hmap f l ++ [hadapt f (l, a)].
+  Proof.
+    intros.
+    rewrite hmap_app.
+    fequal.
+    rewrite hmap_one.
+    unfold preincr, incr, compose.
+    change (@nil B) with (Ƶ: list B) at 1.
+    rewrite monoid_id_l.
+    fequal.
+  Qed.
+
+  (** *** Spec for <<list>> Operations *)
+  (**********************************************************************)
+  Lemma hadapt_nil: forall (a: A),
+    hadapt f (nil, a) = f (nil, a).
+  Proof.
+    reflexivity.
+  Qed.
+
+  Lemma hadapt_cons {a l x}:
+    hadapt f (a :: l, x) =
+      f (f ([], a) :: hmap (f ⦿ [f ([], a)]) l, x).
+  Proof.
+    reflexivity.
+  Qed.
+
+  Lemma hadapt_app {l1 l2 x}:
+    hadapt f (l1 ++ l2, x) =
+      f (hmap f l1 ++ hmap (f ⦿ hmap f l1) l2, x).
+  Proof.
+    cbn.
+    rewrite hmap_app.
+    reflexivity.
+  Qed.
+
+  Lemma hadapt_one {a x}:
+    hadapt f ([a], x) =
+      f ([f ([], a)], x).
+  Proof.
+    cbn.
+    reflexivity.
+  Qed.
+
+End relate_history_prefix.
+
+(** ** Rewriting Rules *)
+(**********************************************************************)
+Lemma hadapt_spec {A B: Type} (f: list B * A -> B):
+  mapd_list_prefix (hadapt f) =
+    hmap f.
+Proof.
+  ext l.
+  generalize dependent f.
+  induction l; intros.
+  - cbn.
+    reflexivity.
+  - rewrite mapd_list_prefix_rw_cons.
+    rewrite hmap_cons.
+    rewrite hadapt_nil.
+    rewrite <- IHl.
+    fequal.
+    fequal.
+    ext [w a'].
+    cbn.
+    reflexivity.
+Qed.
+
+(** * Folding with context AND history *)
+(**********************************************************************)
+Fixpoint fold_with_ctx_history_rec {A B: Type}
+  (f: list B * list A * A -> B)
+  (hist: list B) (ctx: list A)
+
+  (l: list A): list B :=
+  match l with
+  | nil => nil
+  | cons a rest =>
+      f (hist, ctx, a) ::
+        fold_with_ctx_history_rec f (hist ++ [f (hist, ctx, a)]) (ctx ++ [a]) rest
+  end.
+
+Definition fold_with_ctx_history {A B: Type}
+  (f: list B * list A * A -> B)
+  (l: list A): list B :=
+  fold_with_ctx_history_rec f [] [] l.
+
+Section rw.
+
+  Context {A B: Type}.
+
+  Section basic.
+
+    Context (f: list B * list A * A -> B).
+
+    Lemma fold_with_ctx_history_nil_rec: forall hist ctx,
+        fold_with_ctx_history_rec f hist ctx nil = nil.
+    Proof.
+      reflexivity.
+    Qed.
+
+    Lemma fold_with_ctx_history_cons {a l}:
+      fold_with_ctx_history f (a :: l) =
+        f ([], [], a) :: fold_with_ctx_history_rec f [f ([], [], a)] [a] l.
+    Proof.
+      cbn.
+      reflexivity.
+    Qed.
+
+    Lemma fold_with_ctx_history_one_rec {hist ctx a}:
+      fold_with_ctx_history_rec f hist ctx ([a]) =
+        [f (hist, ctx, a)].
+    Proof.
+      cbn.
+      reflexivity.
+    Qed.
+
+    Lemma fold_with_ctx_history_nil:
+      fold_with_ctx_history f nil = nil.
+    Proof.
+      reflexivity.
+    Qed.
+
+    Lemma fold_with_ctx_history_cons_rec {hist ctx a l}:
+      fold_with_ctx_history_rec f hist ctx (a :: l) =
+        f (hist, ctx, a) :: fold_with_ctx_history_rec f (hist ++ [f (hist, ctx, a)]) (ctx ++ [a]) l.
+    Proof.
+      cbn.
+      reflexivity.
+    Qed.
+
+    Lemma fold_with_ctx_history_one {a}:
+      fold_with_ctx_history f ([a]) =
+        [f ([], [], a)].
+    Proof.
+      cbn.
+      reflexivity.
+    Qed.
+
+  End basic.
+
+  Lemma fold_with_ctx_history_app_rec {l1 l2: list A}:
+    forall (f: list B * list A * A -> B) hist ctx,
+      fold_with_ctx_history_rec f hist ctx (l1 ++ l2) =
+        fold_with_ctx_history_rec f hist ctx l1 ++
+          fold_with_ctx_history_rec f (hist ++ fold_with_ctx_history_rec f hist ctx l1) (ctx ++ l1) l2.
+  Proof.
+    induction l1 as [|a l1 IHl1]; intros.
+    - cbn.
+      do 2 rewrite List.app_nil_r.
+      reflexivity.
+    - rewrite <- List.app_comm_cons.
+      rewrite fold_with_ctx_history_cons_rec.
+      rewrite fold_with_ctx_history_cons_rec.
+      rewrite IHl1.
+      rewrite <- List.app_comm_cons.
+      repeat rewrite <- List.app_assoc.
+      reflexivity.
+  Qed.
+
+  Lemma fold_with_ctx_history_app {l1 l2: list A}:
+    forall (f: list B * list A * A -> B),
+      fold_with_ctx_history f (l1 ++ l2) =
+        fold_with_ctx_history f l1 ++
+          fold_with_ctx_history_rec f (fold_with_ctx_history_rec f [] [] l1) l1 l2.
+  Proof.
+    intros. unfold fold_with_ctx_history.
+    rewrite fold_with_ctx_history_app_rec.
+    rewrite List.app_nil_l.
+    rewrite List.app_nil_l.
+    reflexivity.
+  Qed.
+
+End rw.
