Tealeaves/Backends/Nominal/FV.v
@@ -1,18 +1,18 @@
 From Tealeaves Require Import
   Classes.Kleisli.DecoratedTraversableFunctor
   Kleisli.Theory.DecoratedTraversableFunctor
-  Backends.Nominal.Common.
+  Backends.Nominal.Common.Binding.
 
 Import List.ListNotations.
 
-(** * Free Variables *)
+(** * Nominal Free Variables *)
 (**********************************************************************)
 Section FV.
 
   Context
     {T: Type -> Type}
-      `{Mapdt (list name) T}
-      `{! DecoratedTraversableFunctor (list name) T}.
+    `{Mapdt (list name) T}
+    `{! DecoratedTraversableFunctor (list name) T}.
 
   Definition FV_loc: list name * name -> list name :=
     fun '(ctx, x) => if get_binding ctx x then @nil name else [x].
@@ -25,9 +25,8 @@ Section FV.
 
   Context
     `{ToCtxset (list atom) T}
-      `{! Compat_ToCtxset_Mapdt (list atom) T}
-      `{Traverse T}.
-
+    `{! Compat_ToCtxset_Mapdt (list atom) T}
+    `{Traverse T}.
 
   Import Theory.TraversableFunctor.
   Existing Instance ToSubset_Traverse.
@@ -40,22 +39,26 @@ Section FV.
     intros.
     unfold FV.
     compose near t.
-    rewrite (foldMapd_morphism (M1 := list atom) (M2 := Prop)
-               (A := atom) (T := T) (E := list atom) (ϕ := @element_of list _ _ a)
-               (morphism := Monoid_Morphism_element_list atom a)).
+    rewrite
+      (foldMapd_morphism (M1 := list atom) (M2 := Prop)
+         (A := atom) (T := T) (E := list atom) (ϕ := @element_of list _ _ a)
+         (morphism := Monoid_Morphism_element_list atom a)).
     change (Forany_ctx (T := T) (element_of a ∘ FV_loc) t).
     rewrite forany_ctx_iff.
     exists ctx. exists a. split.
     - assumption.
     - unfold compose, FV_loc.
-      destruct (get_binding_spec ctx a) as [[Case1 rest] | [prefix [postfix [Case2 [ctxspec Hnin]]]]].
-      { rewrite Case1.
+      destruct (get_binding_spec_proof ctx a) as
+        [[H_is_Unbound H_notin] | [prefix [postfix [H_is_Bound [ctxspec Hnin]]]]].
+      { rewrite H_is_Unbound.
         rewrite element_of_list_one.
         reflexivity.
       }
-      { rewrite Case2.
+      { rewrite H_is_Bound.
+        false.
         assert (a ∈ ctx).
-        { subst. autorewrite with tea_list.
+        { subst.
+          autorewrite with tea_list.
           tauto. }
         contradiction.
       }
